Formatting and readaibility improvements.

docs/thesis/examples/Examples.v
@@ -7,12 +7,6 @@ Open Scope list_scope.
 
 Set Contextual Implicit.
 
-Fixpoint append { a : Set } (x0 : list a) (x1 : list a) : list a :=
-           match x0, x1 with
-             | nil, ys => ys
-             | cons x xs, ys => cons x (append xs ys)
-           end.
-
 Fixpoint gt (x0 : nat) (x1 : nat) : bool :=
            match x0, x1 with
              | O, O => false
@@ -30,14 +24,29 @@ Set Implicit Arguments.
 
 Inductive quicksort_acc : list nat -> Set :=
           | quicksort_acc_0 : quicksort_acc nil
-          | quicksort_acc_1 : forall (x : nat) (xs : list nat) , quicksort_acc (filter (gt x) xs) -> quicksort_acc (filter (le x) xs) -> quicksort_acc (cons x xs).
+          | quicksort_acc_1 : forall (x : nat) (xs : list nat) , 
+                               quicksort_acc (filter (gt x) xs) 
+                            -> quicksort_acc (filter (le x) xs) 
+                            -> quicksort_acc (cons x xs).
 
-Theorem quicksort_acc_inv_1_0 : forall (x0 : list nat) (x : nat) (xs : list nat) , quicksort_acc x0 -> (x0 = cons x xs) -> quicksort_acc (filter (gt x) xs) .
-intros x0 x xs H; case H; try (intros; discriminate). intros x' xs' Hcall0 Hcall1 . intros Heq0; injection Heq0. intros Heq0_ctx_0 Heq0_ctx_1. try (rewrite <- Heq0_ctx_0).  try (rewrite <- Heq0_ctx_1). assumption.
+Theorem quicksort_acc_inv_1_0 : 
+  forall (x0 : list nat) (x : nat) (xs : list nat), 
+    quicksort_acc x0 -> (x0 = cons x xs) -> quicksort_acc (filter (gt x) xs).
+Proof.
+intros x0 x xs H; case H; try (intros; discriminate). intros x' xs'
+Hcall0 Hcall1.  intros Heq0; injection Heq0. intros Heq0_ctx_0
+Heq0_ctx_1. try (rewrite <- Heq0_ctx_0).  try (rewrite <-
+Heq0_ctx_1). assumption.
 Defined.
 
-Theorem quicksort_acc_inv_1_1 : forall (x0 : list nat) (x : nat) (xs : list nat) , quicksort_acc x0 -> (x0 = cons x xs) -> quicksort_acc (filter (le x) xs) .
-intros x0 x xs H; case H; try (intros; discriminate). intros x' xs' Hcall0 Hcall1 . intros Heq0; injection Heq0. intros Heq0_ctx_0 Heq0_ctx_1. try (rewrite <- Heq0_ctx_0).  try (rewrite <- Heq0_ctx_1). assumption.
+Theorem quicksort_acc_inv_1_1 : 
+  forall (x0 : list nat) (x : nat) (xs : list nat), 
+    quicksort_acc x0 -> (x0 = cons x xs) -> quicksort_acc (filter (le x) xs).
+Proof.
+intros x0 x xs H; case H; try (intros; discriminate). intros x' xs'
+Hcall0 Hcall1 . intros Heq0; injection Heq0. intros Heq0_ctx_0
+Heq0_ctx_1. try (rewrite <- Heq0_ctx_0).  try (rewrite <-
+Heq0_ctx_1). assumption.
 Defined.
 
 Unset Implicit Arguments.
@@ -45,7 +54,8 @@ Unset Implicit Arguments.
 Fixpoint quicksort (x0 : list nat) (x1 : quicksort_acc x0) : list nat :=
            match x0 as _y0 return (x0 = _y0) -> list nat with
              | nil => fun _h0 => nil
-             | cons x xs => fun _h0 => append (quicksort (filter (gt x) xs) (quicksort_acc_inv_1_0 x1 _h0)) (quicksort (filter (le x) xs) (quicksort_acc_inv_1_1 x1 _h0))
+             | cons x xs => fun _h0 => app (quicksort (filter (gt x) xs) (quicksort_acc_inv_1_0 x1 _h0)) 
+                                           (cons x (quicksort (filter (le x) xs) (quicksort_acc_inv_1_1 x1 _h0)))
            end (refl_equal x0).
 
 End Examples.
